Progress on completeing compiler def of loop_to_word

pancake/proofs/loop_to_wordProofScript.sml
@@ -33,33 +33,33 @@ Definition assigned_vars_def:
   (assigned_vars (Assign n exp) l = insert n () l) /\
   (assigned_vars (Store exp n) l = l) /\
   (assigned_vars (SetGlobal w exp) l = l) /\
-  (assigned_vars (LoadByte n w m) l = insert m () l) /\
-  (assigned_vars (StoreByte n w m) l = l) /\
+  (assigned_vars (LoadByte n m) l = insert m () l) /\
+  (assigned_vars (StoreByte n m) l = l) /\
   (assigned_vars (FFI name n1 n2 n3 n4 live) l = l)
 End
 
 Theorem assigned_vars_acc:
   ∀p l.
-    domain (assigned_vars p l) = domain (assigned_vars p LN) UNION domain l
+    domain (assigned_vars p l) = domain (assigned_vars p LN) ∪ domain l
 Proof
   qsuff_tac ‘∀p (l:num_set) l.
     domain (assigned_vars p l) = domain (assigned_vars p LN) UNION domain l’
-  THEN1 metis_tac []
-  \\ ho_match_mp_tac assigned_vars_ind \\ rw [] \\ fs []
-  \\ ntac 4 (once_asm_rewrite_tac [assigned_vars_def])
-  \\ simp_tac (srw_ss()) [domain_def,AC UNION_COMM UNION_ASSOC,domain_union,
-       domain_insert,LET_THM]
-  \\ every_case_tac
-  \\ simp_tac (srw_ss()) [domain_def,AC UNION_COMM UNION_ASSOC,domain_union,
-       domain_insert,LET_THM]
-  \\ once_rewrite_tac [INSERT_SING_UNION]
-  \\ simp_tac (srw_ss()) [domain_def,AC UNION_COMM UNION_ASSOC,domain_union,
-       domain_insert,LET_THM]
-  \\ rpt (pop_assum (fn th => mp_tac (SIMP_RULE std_ss [] th)))
-  \\ rewrite_tac [AND_IMP_INTRO]
-  \\ disch_then (fn th => ntac 6 (once_rewrite_tac [th]))
-  \\ simp_tac (srw_ss()) [domain_def,AC UNION_COMM UNION_ASSOC,domain_union,
-       domain_insert,LET_THM] \\ fs [EXTENSION] \\ metis_tac []
+  >- metis_tac [] >>
+  ho_match_mp_tac assigned_vars_ind >> rw [] >> fs [] >>
+  ntac 4 (once_asm_rewrite_tac [assigned_vars_def]) >>
+  simp_tac (srw_ss()) [domain_def,AC UNION_COMM UNION_ASSOC,domain_union,
+       domain_insert,LET_THM] >>
+  every_case_tac >>
+  simp_tac (srw_ss()) [domain_def,AC UNION_COMM UNION_ASSOC,domain_union,
+       domain_insert,LET_THM] >>
+  once_rewrite_tac [INSERT_SING_UNION] >>
+  simp_tac (srw_ss()) [domain_def,AC UNION_COMM UNION_ASSOC,domain_union,
+       domain_insert,LET_THM] >>
+  rpt (pop_assum (fn th => mp_tac (SIMP_RULE std_ss [] th))) >>
+  rewrite_tac [AND_IMP_INTRO] >>
+  disch_then (fn th => ntac 6 (once_rewrite_tac [th])) >>
+  simp_tac (srw_ss()) [domain_def,AC UNION_COMM UNION_ASSOC,domain_union,
+       domain_insert,LET_THM] >> fs [EXTENSION] >> metis_tac []
 QED
 
 Definition find_var_def:
@@ -69,19 +69,6 @@ Definition find_var_def:
     | SOME n => (n:num)
 End
 
-Definition toNumSet_def:
-  toNumSet [] = LN ∧
-  toNumSet (n::ns) = insert n () (toNumSet ns)
-End
-
-Definition fromNumSet_def:
-  fromNumSet t = MAP FST (toAList t)
-End
-
-Definition mk_new_cutset_def:
-  mk_new_cutset ctxt (l:num_set) =
-    insert 0 () (toNumSet (MAP (find_var ctxt) (fromNumSet l)))
-End
 
 Definition comp_exp_def :
   (comp_exp ctxt (loopLang$Const w) = wordLang$Const w) /\
@@ -93,32 +80,58 @@ Definition comp_exp_def :
    let wexps = MAP (comp_exp ctxt) wexps in
    Op op wexps)
 Termination
-  WF_REL_TAC ‘measure (loopLang$exp_size (K 0) o SND)’
-  \\ rw []
-  \\ rename [‘MEM x xs’]
-  \\ Induct_on ‘xs’ \\ fs []
-  \\ fs [exp_size_def]
-  \\ rw [] \\ fs []
+  WF_REL_TAC ‘measure (loopLang$exp_size (K 0) o SND)’ >>
+  rw [] >>
+  rename [‘MEM x xs’] >>
+  Induct_on ‘xs’ >> fs [] >>
+  fs [exp_size_def] >>
+  rw [] >> fs []
+End
+
+Definition toNumSet_def:
+  toNumSet [] = LN ∧
+  toNumSet (n::ns) = insert n () (toNumSet ns)
+End
+
+Definition fromNumSet_def:
+  fromNumSet t = MAP FST (toAList t)
+End
+
+(* Why inserting zero? *)
+Definition mk_new_cutset_def:
+  mk_new_cutset ctxt (l:num_set) =
+    insert 0 () (toNumSet (MAP (find_var ctxt) (fromNumSet l)))
 End
 
 Definition comp_def:
-  (comp ctxt (Seq p1 p2) l =
-    let (p1,l) = comp ctxt p1 l in
-    let (p2,l) = comp ctxt p2 l in
-      (wordLang$Seq p1 p2,l)) /\
+  (comp ctxt Skip l = (wordLang$Skip,l)) /\
+  (comp ctxt (Assign n e) l =
+     (Assign (find_var ctxt n) (comp_exp ctxt e),l)) /\
+  (comp ctxt (Store e v) l =
+     (Store (comp_exp ctxt e) (find_var ctxt v), l)) /\
+  (comp ctxt (SetGlobal a e) l =
+     (Set (Temp a) (comp_exp ctxt e), l)) /\
+  (comp ctxt (LoadByte a v) l =
+     (Inst (Mem Load8 v ((Addr a 0w))), l)) /\
+  (comp ctxt (StoreByte a v) l =
+     (Inst (Mem Store8 v ((Addr a 0w))), l)) /\
+  (comp ctxt (Seq p q) l =
+    let (wp,l) = comp ctxt p l in
+     let (wq,l) = comp ctxt q l in
+       (Seq wp wq,l)) /\
+  (comp ctxt (If c n ri p q l1) l =
+    let (wp,l) = comp ctxt p l in
+     let (wq,l) = comp ctxt q l in
+       (Seq (If c n ri wp wq) Tick,l)) /\
+  (comp ctxt (Loop l1 body l2) l = (Skip,l)) /\ (* not present in input *)
   (comp ctxt Break l = (Skip,l)) /\ (* not present in input *)
   (comp ctxt Continue l = (Skip,l)) /\ (* not present in input *)
-  (comp ctxt (Loop l1 body l2) l = (Skip,l)) /\ (* not present in input *)
-  (comp ctxt (If x1 x2 x3 p1 p2 l1) l =
-    let (p1,l) = comp ctxt p1 l in
-    let (p2,l) = comp ctxt p2 l in
-      (Seq (If x1 x2 x3 p1 p2) Tick,l)) /\
-  (comp ctxt (Mark p1) l = comp ctxt p1 l) /\
-  (comp ctxt Tick l = (Tick,l)) /\
-  (comp ctxt Skip l = (Skip,l)) /\
-  (comp ctxt Fail l = (Skip,l)) /\
   (comp ctxt (Raise v) l = (Raise (find_var ctxt v),l)) /\
   (comp ctxt (Return v) l = (Return 0 (find_var ctxt v),l)) /\
+  (comp ctxt Tick l = (Tick,l)) /\
+  (comp ctxt (Mark p) l = comp ctxt p l) /\
+  (comp ctxt Fail l = (Skip,l)) /\
+  (comp ctxt (LocValue n m) l = (LocValue (find_var ctxt n) m,l))  /\
   (comp ctxt (Call ret dest args handler) l =
      let args = MAP (find_var ctxt) args in
        case ret of
@@ -135,14 +148,12 @@ Definition comp_def:
               let new_l = (FST l1, SND l1+1) in
                 (Seq (Call (SOME (v,live,p2,l)) dest args
                    (SOME (find_var ctxt n,p1,l1))) Tick, new_l)) /\
-  (comp ctxt (LocValue n m) l = (LocValue (find_var ctxt n) m,l))  /\
-  (comp ctxt (Assign n exp) l = (Assign (find_var ctxt n) (comp_exp ctxt exp),l)) /\
-  (comp ctxt (Store exp v) l = (Store (comp_exp ctxt exp) (find_var ctxt v), l)) /\
-  (comp ctxt (FFI name n1 n2 n3 n4 live) l =
-   (FFI name (find_var ctxt n1) (find_var ctxt n2) (find_var ctxt n3) (find_var ctxt n4) live,l)) /\
-  (comp ctxt prog l = (Skip,l))
+   (comp ctxt (FFI f ptr1 len1 ptr2 len2 live) l =
+     (FFI f (find_var ctxt len1) (find_var ctxt ptr2)
+      (find_var ctxt len2) (find_var ctxt len2) live,l))
 End
 
+(* what is make context? from here *)
 Definition make_ctxt_def:
   make_ctxt n [] l = l ∧
   make_ctxt n (x::xs) l = make_ctxt (n+2:num) xs (insert x n l)
